steel/Zeta.Steel.Main.fsti
@@ -21,12 +21,18 @@ module V = Zeta.Steel.Verifier
 module SA = Zeta.SeqAux
 #push-options "--ide_id_info_off"
 
+let thread_inv_predicate
+  (t:V.thread_state_t)
+  (mlogs:TLM.t)
+  : M.thread_state_model -> vprop
+  = fun tsm ->
+    V.thread_state_inv t tsm `star`
+    TLM.tid_pts_to mlogs tsm.M.thread_id half tsm.M.processed_entries false
+
 let thread_inv (t: V.thread_state_t)
                (mlogs: TLM.t)
   : vprop
-  = exists_ (fun tsm ->
-       V.thread_state_inv t tsm `star`
-       TLM.tid_pts_to mlogs tsm.M.thread_id half tsm.M.processed_entries false)
+  = exists_ (thread_inv_predicate t mlogs)
 
 noeq
 type thread_state (mlogs:TLM.t) =
@@ -85,6 +91,38 @@ val init (_:unit)
         (fun t -> core_inv t `star`
                TLM.tids_pts_to t.aeh.mlogs half (Map.const (Some Seq.empty)) false)
 
+let verify_post
+  (t:top_level_state)
+  (tid:tid)
+  (entries:erased AEH.log)
+  (log_perm:perm)
+  (log_bytes:erased bytes)
+  (len: U32.t)
+  (input:larray U8.t len)
+  (out_len: U32.t)
+  (out_bytes:erased bytes)
+  (output:larray U8.t out_len)
+  : post_t (v:V.verify_result { V.verify_result_complete len v })
+  = fun res ->
+    core_inv t `star`
+    A.pts_to input log_perm log_bytes `star`
+    (match res with
+     | V.Verify_success read wrote ->
+       exists_ (fun entries' ->
+       exists_ (fun out_bytes' ->
+         TLM.tid_pts_to t.aeh.mlogs tid half (entries `Seq.append` entries') false
+           `star`
+         A.pts_to output full_perm out_bytes'
+           `star`
+         pure (V.parse_log_up_to log_bytes (U32.v read) == Some entries' /\
+               (let tsm = M.verify_model (M.init_thread_state_model tid) entries in
+                let tsm' = M.verify_model tsm entries' in
+                Application.n_out_bytes tsm tsm' wrote out_bytes out_bytes'))))
+
+     | _ ->
+       exists_ (A.pts_to output full_perm) `star`
+       exists_ (fun entries' -> TLM.tid_pts_to t.aeh.mlogs tid half entries' false))
+
 val verify_log (t:top_level_state)
                (tid:tid)
                (#entries:erased AEH.log)
@@ -100,26 +138,7 @@ val verify_log (t:top_level_state)
      A.pts_to input log_perm log_bytes `star`
      A.pts_to output full_perm out_bytes `star`
      TLM.tid_pts_to t.aeh.mlogs tid half entries false)
-    (fun res ->
-      core_inv t `star`
-      A.pts_to input log_perm log_bytes `star`
-      (match res with
-       | V.Verify_success read wrote ->
-         exists_ (fun entries' ->
-         exists_ (fun out_bytes' ->
-           TLM.tid_pts_to t.aeh.mlogs tid half
-                          (entries `Seq.append` entries')
-                          false `star`
-           A.pts_to output full_perm out_bytes' `star`
-           pure (V.parse_log_up_to log_bytes (U32.v read) == Some entries' /\
-                (let tsm = M.verify_model (M.init_thread_state_model tid) entries in
-                 let tsm' = M.verify_model tsm entries' in
-                 Application.n_out_bytes tsm tsm' wrote out_bytes out_bytes'))))
-
-       | _ ->
-         exists_ (A.pts_to output full_perm) `star`
-         exists_ (fun entries' ->
-                    TLM.tid_pts_to t.aeh.mlogs tid half entries' false)))
+    (verify_post t tid entries log_perm log_bytes len input out_len out_bytes output)
 
 let max_certified_epoch (t:top_level_state)
   : STT (option M.epoch_id)
